...내가 왜 'Zero'가 이미 정의되어 있는 것을 떠올리지 못했지...?

src/lean/Nemonuri/Study/StanfordOnline/Compilers/Introduction/Basic.lean
@@ -9,17 +9,11 @@ public section public_s
 
 set_option autoImplicit false
 
+
+
+
 namespace Nemonuri.Study.StanfordOnline.Compilers
 
-/-
-universe u v
-
-structure State (St: Type u) where val: St
-
-structure Label (La: Type v) where val: La
-
-def LTS (St: Type u) (La: Type v) := Cslib.LTS (State St) (Label La)
--/
 
 universe us ul
 
@@ -28,20 +22,35 @@ class LabelMorph (LabelA LabelB: Type _)
   extends
     SetLike LabelA (List (Option LabelB))
 
-
 /-
-instance (priority := low) (Label1 Label2: Type ul) : LabelMap Label1 Label2 where
-  labelMap _ := .none
--/
+class LtsM (St La: Type _)
+  extends
+    Cslib.LTS St La
 
---def LabelMap.toMorphism {Label1 Label2 State} (inst: LabelMap Label1 Label2)
-/-
-def LabelMap.mapLTS {St} (La1 La2) [LabelMap La1 La2] (lts: Cslib.LTS St La1) : Cslib.LTS St (Option La2) :=
-  { Tr st1 la2? st2 :=
-      ∀(la1: La1), ((LabelMap.labelMap la1) = la2?) → (la2?.isSome) → (lts.Tr st1 la1 st2) }
+def _root_.Cslib.LTS.map {St LaB} (lts: Cslib.LTS St LaB) [LtsM St LaB] LaA [LabelMorph LaA LaB] : Cslib.LTS St LaA :=
+  lts.mapByLabelMorph LaA
+
+theorem LtsM.map_eq
+  {St LaB} (lts: Cslib.LTS St LaB) [LtsM St LaB] LaA [LabelMorph LaA LaB] st1 laa st2
+  : (LtsM.map lts).Tr st1 laa st2
 -/
 
 end Nemonuri.Study.StanfordOnline.Compilers
+
+def Cslib.LTS.mapByLabelMorph {St LaB} (ltsB: Cslib.LTS St LaB) LaA [SetLike LaA (List (Option LaB))] : Cslib.LTS St LaA :=
+  { Tr st1 la st2 := ∀lb, (lb ∈ SetLike.coe la) → ltsB.withIdle.MTr st1 lb st2 }
+
+open Nemonuri.Study.StanfordOnline.Compilers in
+def Cslib.LTS.mapTo {St LaB} (ltsB: Cslib.LTS St LaB) LaA [LabelMorph LaA LaB] : Cslib.LTS St LaA :=
+  ltsB.mapByLabelMorph LaA
+
+
+open Nemonuri.Study.StanfordOnline.Compilers Cslib.LTS in
+theorem Cslib.LTS.mapTo_iff {St LaB} (ltsB: Cslib.LTS St LaB) LaA [lm: LabelMorph LaA LaB] st1 la st2
+  : (Cslib.LTS.mapTo ltsB LaA).Tr st1 la st2 ↔ (∀lb, ((lm.coe la lb) → ltsB.withIdle.MTr st1 lb st2)) := by
+  simp [mapTo]
+  simp [mapByLabelMorph]
+  simp [Membership.mem, Set.Mem]
 
 /-
 open Nemonuri.Study.StanfordOnline.Compilers in
@@ -50,9 +59,6 @@ def Cslib.LTS.mapByLabelMap {St La1} (lts: Cslib.LTS St La1) La2 [LabelMap La1 L
       ∀(la1: La1), ((LabelMap.labelMap la1) = la2?) → (la2?.isSome) → (lts.Tr st1 la1 st2) }
 -/
 
-open Nemonuri.Study.StanfordOnline.Compilers in
-def Cslib.LTS.mapByLabelMorph {St LaB} (ltsB: Cslib.LTS St LaB) LaA [LabelMorph LaA LaB] : Cslib.LTS St LaA :=
-  { Tr st1 la st2 := ∀lb, (lb ∈ SetLike.coe la) → ltsB.withIdle.MTr st1 lb st2 }
 
 theorem Cslib.LTS.MTr.single_iff.{u, v}
   {State : Type u} {Label : Type v} (lts : LTS State Label) (s1 : State) (μ : Label) (s2 : State)
